GoldbachTm/Tm27/Content.lean
@@ -9,7 +9,7 @@ theorem lemma_26 (n : ℕ) (i : ℕ)
 (even_n : Even (n+2))
 (g :
 nth_cfg i = some ⟨⟨26, by omega⟩, ⟨Γ.zero, Turing.ListBlank.mk (List.replicate (n+4) Γ.one), Turing.ListBlank.mk []⟩⟩ )
-( hpp : goldbach (n+4)) :
+( hpp : Goldbach (n+4)) :
 ∃ j>i, nth_cfg j = some ⟨⟨26, by omega⟩, ⟨Γ.zero, Turing.ListBlank.mk (List.replicate (n+4+2) Γ.one), Turing.ListBlank.mk []⟩⟩
 := by
 forward g
@@ -39,7 +39,7 @@ refine (?_ ∘ g) ?_
     omega
 
 lemma never_halt_step (n : ℕ) :
-(∀ i < n, goldbach (2*i+4)) ->
+(∀ i < n, Goldbach (2*i+4)) ->
 ∃ j, nth_cfg j = some ⟨⟨26, by omega⟩, ⟨Γ.zero, Turing.ListBlank.mk (List.replicate (2*n+4) Γ.one), Turing.ListBlank.mk []⟩⟩
  := by
 induction n with
@@ -67,7 +67,7 @@ refine (?_ ∘ induction_step) ?_
   apply h i (by omega)
 
 theorem never_halt (never_none : ∀ i, nth_cfg i ≠ none) (n : ℕ):
-goldbach (2*n + 4)
+Goldbach (2*n + 4)
 := by
 induction' n using Nat.strongRecOn with n IH
 apply never_halt_step at IH
@@ -87,7 +87,7 @@ refine (?_ ∘ g) ?_
   tauto
 
 
-theorem halt_lemma_rev' (h : ∀ n, goldbach (2*n+4)) :
+theorem halt_lemma_rev' (h : ∀ n, Goldbach (2*n+4)) :
 ∀ i, nth_cfg i ≠ none := by
 apply propagating_induction (fun i => nth_cfg i ≠ none) (fun i n => nth_cfg i = some ⟨⟨26, by omega⟩, ⟨Γ.zero, Turing.ListBlank.mk (List.replicate (2*n+4) Γ.one), Turing.ListBlank.mk []⟩⟩) 45
 . simp [cfg45]; tauto
@@ -112,11 +112,11 @@ apply propagating_induction (fun i => nth_cfg i ≠ none) (fun i n => nth_cfg i 
   tauto
 
 theorem halt_lemma':
-(∃ n, ¬ goldbach (2*n+4)) → (∃ i, nth_cfg i = none)
+(∃ n, ¬ Goldbach (2*n+4)) → (∃ i, nth_cfg i = none)
 := by
 intros h
 obtain ⟨j, hj⟩ := never_halt_step (Nat.find h) (λ i g =>
-by rw [← Mathlib.Tactic.PushNeg.not_not_eq (goldbach (2*i+4))]
+by rw [← Mathlib.Tactic.PushNeg.not_not_eq (Goldbach (2*i+4))]
    apply Nat.find_min h g
 )
 forward hj
@@ -129,7 +129,7 @@ apply Nat.find_spec h
 use! x, y
 
 theorem halt_lemma_rev :
-(∃ i, nth_cfg i = none) → (∃ n, ¬ goldbach (2*n+4))
+(∃ i, nth_cfg i = none) → (∃ n, ¬ Goldbach (2*n+4))
 := by
 intros h
 by_contra! g
